src/Implementations/File/FileInnerSpecs.v
@@ -1,0 +1,881 @@
+Require Import Framework FSParameters AuthenticatedDiskLayer.
+Require Import BlockAllocator Inode File.
+Require Import Compare_dec FunctionalExtensionality Lia.
+Import IfNotations.
+
+
+(*** Lemmas ***)
+
+Ltac solve_bounds:=
+  match goal with
+  |[H: forall _: nat , _ -> ?x _ = _ |- ?x _ = _ ] =>
+   pose proof inodes_before_data;
+   rewrite H;
+   unfold DiskAllocatorParams.bitmap_addr,
+   DiskAllocatorParams.num_of_blocks,
+   InodeAllocatorParams.bitmap_addr,
+   InodeAllocatorParams.num_of_blocks in *;
+   try lia; eauto
+  end.
+
+
+Set Nested Proofs Allowed.
+Lemma inode_rep_some_inbounds:
+forall im s inum inode,
+inode_rep im s ->
+im inum = Some inode ->
+inum < inode_count.
+Proof.
+unfold inode_rep, block_allocator_rep,
+inode_map_rep, inode_map_valid,
+InodeAllocatorParams.num_of_blocks; intros; cleanup.
+destruct (lt_dec inum inode_count); eauto.
+rewrite H1, H6 in H0; 
+simpl in *; try congruence; try lia.
+Qed.
+
+Lemma inode_exists_then_file_exists:
+  forall fm im s inum inode,
+  file_map_rep fm im s ->
+  im inum = Some inode ->
+  exists f, fm inum = Some f.
+Proof.
+  unfold file_map_rep; intros; cleanup.
+  destruct_fresh (fm inum); eauto.
+  edestruct H; exfalso.
+  apply H3; eauto; congruence.
+Qed.
+
+Lemma inode_missing_then_file_missing:
+  forall fm im s inum,
+  file_map_rep fm im s ->
+  im inum = None ->
+  fm inum = None.
+Proof.
+  unfold file_map_rep, addrs_match_exactly; intros; cleanup.
+  destruct_fresh (fm inum); eauto.
+  edestruct H; exfalso.
+  eapply H2; eauto; congruence.
+Qed.
+
+Lemma Some_injective:
+  forall A (a1 a2: A),
+    Some a1 = Some a2 ->
+    a1 = a2.
+Proof.
+  intros; congruence.
+Qed.
+
+Lemma nth_error_updN_eq:
+  forall T (l: list T) n m v,
+    n = m ->
+    n < length l ->
+    nth_error (updN l n v) m = Some v.
+Proof.
+  induction l; simpl; intros; eauto.
+  lia.
+  destruct n; simpl in *; 
+  cleanup; simpl in *; eauto.
+  rewrite IHl; eauto; lia.
+Qed.
+
+Lemma nth_error_updN_ne:
+  forall T (l: list T) n m v,
+    n <> m \/ n >= length l ->
+    nth_error (updN l n v) m = nth_error l m.
+Proof.
+  induction l; simpl; intros; eauto.
+  destruct n; simpl in *;
+  cleanup; simpl in *; eauto.
+  split_ors; cleanup; try lia.
+  destruct m; simpl in *; eauto; lia.
+  destruct m; simpl; eauto.
+  rewrite IHl; eauto; lia.
+Qed.
+
+Lemma selN_not_In_ne:
+  forall T (l: list T) a t def,
+  ~In t l ->
+  a < length l ->
+  t <> selN l a def.
+  Proof.
+  induction l; simpl; intros; eauto.
+  lia.
+  destruct a0; eauto.
+  eapply IHl; eauto; lia.
+  Qed.
+
+
+Lemma NoDup_selN_ne:
+  forall T (l: list T) a b def1 def2,
+    NoDup l ->
+    a < length l ->
+    b < length l ->
+    a <> b ->
+    selN l a def1 <> selN l b def2.
+Proof.
+  induction l; simpl; intros; eauto.
+  lia.
+  inversion H; cleanup; clear H.
+  destruct a0, b; simpl in *;
+  cleanup; simpl in *; eauto; try lia.
+  eapply selN_not_In_ne; eauto; lia.
+  intros Hnot; 
+  symmetry in Hnot; 
+  eapply selN_not_In_ne; 
+  eauto; lia.
+  eapply IHl; eauto; lia.
+Qed.
+
+Lemma files_inner_rep_eq:
+  forall fd1 fd2 s,
+    files_inner_rep fd1 s ->
+    files_inner_rep fd2 s ->
+    fd1 = fd2.
+Proof.
+  unfold files_rep, files_inner_rep;
+  intros; extensionality inum.
+  cleanup.
+  eapply DiskAllocator.block_allocator_rep_eq in H3; eauto; subst.
+  eapply inode_rep_eq in H; eauto; subst.
+  unfold file_map_rep in *; cleanup.
+  unfold addrs_match_exactly in *.
+  specialize (H inum); specialize (H3 inum);
+  destruct_fresh (fd1 inum); cleanup;
+  destruct_fresh (x0 inum).
+  {
+    destruct_fresh (fd2 inum).
+    {
+      eapply_fresh H2 in D0; eauto.
+      eapply_fresh H4 in D0; eauto.
+      unfold file_rep in *; cleanup.
+      destruct f, f0; simpl in *; cleanup.
+      assert_fresh (blocks = blocks0). {
+        eapply list_selN_ext'; eauto.
+        intros.
+        repeat rewrite nth_selN_eq.
+        apply Some_injective.
+        repeat rewrite <- nth_error_nth'; try lia.
+        destruct_fresh (nth_error (block_numbers i) pos).
+        eapply_fresh H7 in D2; eauto; cleanup.
+        eapply_fresh H10 in D2; eauto; cleanup; eauto.
+        apply nth_error_None in D2; lia.
+      }
+      rewrite A; eauto.
+    }
+    {
+      edestruct H; eauto.
+      exfalso; eapply H6; congruence.
+    }
+  }
+  {
+    edestruct H3; eauto.
+    exfalso; eapply H5; congruence.
+  }
+  {
+    edestruct H3; eauto.
+    exfalso; eapply H6; congruence.
+  }
+  {
+    destruct_fresh (fd2 inum); eauto.
+    {
+      edestruct H; eauto.
+      exfalso; eapply H5; congruence.
+    }
+  }
+  Unshelve.
+  exact value0.
+Qed.
+
+Lemma files_rep_eq:
+  forall fd1 fd2 s,
+    files_rep fd1 s ->
+    files_rep fd2 s ->
+    fd1 = fd2.
+Proof.
+  unfold files_rep; intros; cleanup.
+  eapply files_inner_rep_eq in H2; eauto.
+Qed.
+
+Lemma files_crash_rep_eq:
+  forall fd1 fd2 s,
+    files_crash_rep fd1 s ->
+    files_crash_rep fd2 s ->
+    fd1 = fd2.
+Proof.
+  unfold files_crash_rep; intros; cleanup.
+  eapply files_inner_rep_eq in H; eauto.
+Qed.
+
+
+
+(*** Inner Finished Specs ***)
+
+Lemma free_all_blocks_finished:
+  forall u l_a o s s' r block_map,
+    DiskAllocator.block_allocator_rep block_map (fst s) ->
+    exec (TransactionalDiskLang data_length) u o s (free_all_blocks l_a) (Finished s' r) ->
+    exists new_block_map,
+    ((r = None /\
+     DiskAllocator.block_allocator_rep new_block_map (fst s')) \/
+    (r = Some tt /\
+     DiskAllocator.block_allocator_rep new_block_map (fst s') /\
+     (forall a, In a l_a -> new_block_map a = None))) /\
+    (forall a,
+       a < DiskAllocatorParams.bitmap_addr \/
+       a > DiskAllocatorParams.bitmap_addr + DiskAllocatorParams.num_of_blocks -> 
+       fst s' a = fst s a) /\
+    (forall a, ~In a l_a -> new_block_map a = block_map a) /\
+    snd s' = snd s.
+Proof.
+  induction l_a; simpl; intros; eauto.
+  invert_exec; eexists; intuition eauto.
+
+  cleanup; repeat invert_exec.
+  {
+    eapply DiskAllocator.free_finished in H0; eauto.
+    cleanup; split_ors; cleanup.
+    eapply IHl_a in H1; eauto.
+    cleanup; split_ors; cleanup.
+    {
+      eexists; intuition eauto.
+      rewrite H1; eauto.
+      rewrite H1; eauto.
+      rewrite H5; eauto.
+      rewrite Mem.delete_ne; eauto.
+    }
+    {
+      exists x.
+      intuition eauto.      
+      right; intuition eauto.
+      subst.
+      destruct (in_dec addr_dec a0 l_a); eauto.
+      rewrite H5; eauto.
+      rewrite Mem.delete_eq; eauto.
+      rewrite H1; eauto.
+      rewrite H1; eauto.
+      rewrite H5; eauto.
+      rewrite Mem.delete_ne; eauto.
+    }
+  }
+  {
+    eapply DiskAllocator.free_finished in H0; eauto.
+    cleanup; split_ors; cleanup.
+    eexists; intuition eauto.
+  }
+Qed.
+
+Lemma change_owner_inner_finished:
+  forall u s s' o t own inum fm,
+    files_inner_rep fm (fst s) ->
+    exec (TransactionalDiskLang data_length) u o s (change_owner_inner own inum) (Finished s' t) ->
+    (t = None \/
+      (exists f, 
+      fm inum = Some f /\
+      files_inner_rep (Mem.upd fm inum (change_file_owner f own)) (fst s'))) /\
+      snd s' = snd s.
+Proof.
+  unfold change_owner_inner; intros; repeat invert_exec_no_match.
+  unfold files_rep, files_inner_rep in *; simpl in *; cleanup_no_match.
+  repeat cleanup_pairs.
+  eapply Inode.change_owner_finished in H0; eauto.
+
+  simpl in *; cleanup_no_match; split_ors; cleanup_no_match;
+  repeat cleanup_pairs; repeat invert_exec_no_match; intuition eauto.
+
+    eapply_fresh inode_exists_then_file_exists in H4; eauto; cleanup.
+    unfold file_map_rep in *; cleanup.
+    eapply_fresh H6 in H4; eauto.
+    unfold file_rep in *; cleanup; eauto.
+    right; eexists; intuition eauto.
+    eexists; intuition eauto.
+    eexists; intuition eauto.
+    eapply DiskAllocator.block_allocator_rep_inbounds_eq; eauto;
+    intros; repeat solve_bounds.
+    {
+        unfold addrs_match_exactly in *; intros.
+        destruct (addr_dec inum a); subst.
+        repeat rewrite Mem.upd_eq; eauto.
+        split; intros; congruence.
+        repeat rewrite Mem.upd_ne; eauto.
+    }
+    all:
+    destruct (addr_dec inum inum0); subst;
+    [rewrite Mem.upd_eq in H10;
+        rewrite Mem.upd_eq in H11; eauto |
+        rewrite Mem.upd_ne in H10;
+        rewrite Mem.upd_ne in H11; eauto];
+    cleanup; simpl; eauto;
+    eapply H6 in H10; eauto; cleanup; eauto.
+Qed. 
+
+Lemma delete_inner_finished:
+  forall u s s' o t inum fm,
+    files_inner_rep fm (fst s) ->
+    exec (TransactionalDiskLang data_length) u o s (delete_inner inum) (Finished s' t) ->
+    (t = None \/
+      (files_inner_rep (Mem.delete fm inum) (fst s'))) /\
+      snd s' = snd s.
+Proof.
+  unfold delete_inner; intros; repeat invert_exec_no_match.
+  unfold files_rep, files_inner_rep in *; simpl in *; cleanup_no_match.
+  repeat cleanup_pairs.
+  eapply get_all_block_numbers_finished in H0; eauto.
+  simpl in *; cleanup_no_match; split_ors; cleanup_no_match;
+  repeat cleanup_pairs; repeat invert_exec_no_match; eauto.
+
+  eapply free_all_blocks_finished in H0; eauto.
+  2: eapply DiskAllocator.block_allocator_rep_inbounds_eq; eauto;
+  intros; repeat solve_bounds.
+
+  simpl in *; cleanup_no_match; split_ors; cleanup_no_match;
+  repeat cleanup_pairs; repeat invert_exec_no_match; try solve [intuition eauto].
+  unfold inode_rep in *; cleanup.
+  eapply free_finished in H1; eauto.
+  2: simpl; eexists; intuition eauto;
+  eapply InodeAllocator.block_allocator_rep_inbounds_eq; eauto;
+  intros; repeat solve_bounds.
+
+  simpl in *; cleanup_no_match; split_ors; cleanup_no_match;
+  repeat cleanup_pairs; repeat invert_exec_no_match; intuition eauto.
+  {
+
+    eapply_fresh inode_exists_then_file_exists in H6; eauto; cleanup.
+    unfold file_map_rep in *; cleanup.
+    eapply_fresh H14 in H6; eauto.
+    unfold file_rep in *; cleanup; eauto.
+    right; eexists; intuition eauto.
+    eexists; intuition eauto.
+    eapply DiskAllocator.block_allocator_rep_inbounds_eq; eauto;
+    intros; repeat solve_bounds.
+          {
+            unfold addrs_match_exactly in *; intros.
+            destruct (addr_dec inum a); subst.
+            repeat rewrite Mem.delete_eq; eauto.
+            split; intros; congruence.
+            repeat rewrite Mem.delete_ne; eauto.
+          }
+          {
+            destruct (addr_dec inum inum0); subst;
+            [rewrite Mem.delete_eq in H18;
+             rewrite Mem.delete_eq in H19; eauto |
+             rewrite Mem.delete_ne in H18;
+             rewrite Mem.delete_ne in H19; eauto];
+            try congruence.
+            eapply_fresh H14 in H18; eauto.
+            unfold file_rep in *; cleanup; eauto.
+          }
+          {
+            destruct (addr_dec inum inum0); subst;
+            [rewrite Mem.delete_eq in H18;
+             rewrite Mem.delete_eq in H19; eauto |
+             rewrite Mem.delete_ne in H18;
+             rewrite Mem.delete_ne in H19; eauto];
+            try congruence.
+            eapply_fresh H14 in H18; eauto.
+            unfold file_rep in *; cleanup; eauto.
+          }
+          {
+            destruct (addr_dec inum inum0); subst;
+            [rewrite Mem.delete_eq in H18;
+             rewrite Mem.delete_eq in H19; eauto |
+             rewrite Mem.delete_ne in H18;
+             rewrite Mem.delete_ne in H19; eauto];
+            try congruence.
+            {
+              unfold inode_map_rep,
+              inode_map_valid in *;
+              cleanup.
+              eapply H24 in H6; eauto.
+              cleanup.
+              eapply_fresh H14 in H18; eauto;
+              cleanup.
+              unfold file_rep; simpl;
+              intuition eauto.
+              eapply_fresh H25 in H20; cleanup.
+              eexists; intuition eauto.
+              eapply nth_error_In in H20.
+              eapply not_In_NoDup_app in H20; eauto.
+              rewrite H8; eauto.
+            }
+          }
+        }
+Qed. 
+
+Lemma extend_inner_finished:
+  forall u s s' o t inum v fm,
+    files_inner_rep fm (fst s) ->
+    
+    exec (TransactionalDiskLang data_length) u o s (extend_inner v inum) (Finished s' t) ->
+    (t = None \/
+      (exists f, 
+      fm inum = Some f /\
+      files_inner_rep (Mem.upd fm inum (extend_file f v)) (fst s'))) /\
+      snd s' = snd s.
+Proof.
+  unfold extend_inner; intros; repeat invert_exec_no_match.
+  unfold files_rep, files_inner_rep in *; simpl in *; cleanup_no_match.
+  repeat cleanup_pairs.
+  eapply DiskAllocator.alloc_finished in H0; eauto.
+  simpl in *; cleanup_no_match; split_ors; cleanup_no_match;
+  repeat cleanup_pairs; repeat invert_exec_no_match; eauto.
+
+  unfold inode_rep in *; cleanup.
+  eapply Inode.extend_finished in H1; eauto.
+  2: simpl; eexists; intuition eauto; 
+  eapply InodeAllocator.block_allocator_rep_inbounds_eq; eauto;
+  intros; repeat solve_bounds.
+
+  simpl in *; cleanup_no_match; split_ors; cleanup_no_match;
+  repeat cleanup_pairs; repeat invert_exec_no_match; intuition eauto.
+  {
+
+  eapply_fresh inode_exists_then_file_exists in H9; eauto; cleanup.
+    unfold file_map_rep in *; cleanup.
+      eapply_fresh H11 in H9; eauto.
+      unfold file_rep in *; cleanup; eauto.
+                
+        right; eexists; intuition eauto.
+        eexists; intuition eauto.
+        eexists; intuition eauto.
+        eapply DiskAllocator.block_allocator_rep_inbounds_eq; eauto.
+        intros; repeat solve_bounds.
+          {
+            unfold addrs_match_exactly in *; intros.
+            destruct (addr_dec inum a); subst.
+            repeat rewrite Mem.upd_eq; eauto.
+            split; intros; congruence.
+            repeat rewrite Mem.upd_ne; eauto.
+          }
+          {
+            destruct (addr_dec inum inum0); subst;
+            [rewrite Mem.upd_eq in H15;
+             rewrite Mem.upd_eq in H16; eauto |
+             rewrite Mem.upd_ne in H15;
+             rewrite Mem.upd_ne in H16;eauto].
+            {
+              cleanup; simpl; intuition eauto.
+            }
+            {
+              eapply H11 in H15; eauto; cleanup; eauto.
+            }
+          }
+          {
+            destruct (addr_dec inum inum0); subst;
+            [rewrite Mem.upd_eq in H15;
+             rewrite Mem.upd_eq in H16; eauto |
+             rewrite Mem.upd_ne in H15;
+             rewrite Mem.upd_ne in H16;eauto].
+            
+            - cleanup; simpl; repeat rewrite app_length; simpl; eauto.
+            
+            - eapply H11 in H15; eauto; cleanup; eauto.
+          }
+          {
+            destruct (addr_dec inum inum0); subst;
+            [rewrite Mem.upd_eq in H15;
+           rewrite Mem.upd_eq in H16; eauto |
+           rewrite Mem.upd_ne in H15;
+           rewrite Mem.upd_ne in H16;eauto].
+          {
+            cleanup; simpl in *.
+              destruct (lt_dec i (length x5.(blocks))).
+              - rewrite nth_error_app1 in H17; eauto.
+                apply H14 in H17; cleanup.
+                eexists; rewrite nth_error_app1; eauto.
+                split; eauto.
+                rewrite Mem.upd_ne; eauto.
+                intros Hnot; subst; congruence.
+                lia.
+                lia.
+
+              - assert (A: i = length x5.(blocks)). {
+                  apply nth_error_some_lt in H17;
+                  rewrite app_length in H17; simpl in *;
+                  lia.
+                }
+                subst.
+                rewrite nth_error_app2 in *; try lia.
+                rewrite H13 in *.
+                rewrite PeanoNat.Nat.sub_diag in *; simpl in *.
+                cleanup; eexists; intuition eauto.
+                rewrite Mem.upd_eq; eauto.
+            }
+            {
+              eapply_fresh H11 in H15; eauto; cleanup.
+              unfold file_rep; simpl;
+              intuition eauto.
+              eapply H20 in H17; cleanup.
+              eexists; intuition eauto.
+              rewrite Mem.upd_ne; eauto.
+              intros Hnot; subst; congruence.
+            }
+          }
+        }
+        {
+          intros.
+          eapply_fresh inode_exists_then_file_exists in H8; 
+          eauto; cleanup.
+         unfold file_map_rep in *; cleanup.
+         eapply_fresh H10 in H8; eauto.
+         unfold file_rep in *; cleanup; eauto.
+         intros Hnot; apply In_nth_error in Hnot; cleanup.
+         apply H13 in H14; cleanup; congruence.
+      }
+  Qed.
+
+
+Lemma write_inner_finished:
+  forall u s s' o t inum off v fm,
+    files_inner_rep fm (fst s) ->
+    
+    exec (TransactionalDiskLang data_length) u o s (write_inner off v inum) (Finished s' t) ->
+    (t = None \/
+      (exists f, 
+      fm inum = Some f /\
+      off < length f.(blocks) /\
+      files_inner_rep (Mem.upd fm inum (update_file f off v)) (fst s'))) /\
+      snd s' = snd s.
+Proof.
+  unfold write_inner; intros; repeat invert_exec_no_match.
+  unfold files_rep, files_inner_rep in *; simpl in *; cleanup_no_match.
+  repeat cleanup_pairs.
+  eapply get_block_number_finished in H0; eauto.
+  simpl in *; cleanup_no_match; split_ors; cleanup_no_match;
+  repeat cleanup_pairs; repeat invert_exec_no_match;
+  eapply_fresh DiskAllocator.block_allocator_rep_inbounds_eq with (s2 := t1) in H2.
+  all: try solve [intros; repeat solve_bounds].
+  {
+    eapply DiskAllocator.write_finished in H1; eauto.
+  simpl in *; cleanup_no_match; split_ors; cleanup_no_match;
+  repeat cleanup_pairs; repeat invert_exec_no_match; intuition eauto.
+
+  simpl; repeat (split; eauto).  
+  eapply_fresh inode_exists_then_file_exists in H7; eauto; cleanup.
+  unfold inode_rep in *; cleanup_no_match;
+  right; eexists; intuition eauto; cleanup; eauto.
+  {
+    unfold file_map_rep, file_rep in *; cleanup.
+    eapply H11 in H7; eauto; cleanup; lia.
+  }
+  eexists; intuition eauto.
+  eexists; intuition eauto.
+  eapply InodeAllocator.block_allocator_rep_inbounds_eq; [eauto | intros; repeat solve_bounds].
+  eexists; split; [ |eauto]; eauto.
+  unfold file_map_rep in *; cleanup.
+  intuition eauto.  
+  {
+    unfold addrs_match_exactly in *; intros.
+    destruct (addr_dec inum a); subst.
+    rewrite Mem.upd_eq; eauto.
+    split; intros; congruence.
+    rewrite Mem.upd_ne; eauto.
+  }
+  {
+    destruct (addr_dec inum inum0); subst;
+    [rewrite Mem.upd_eq in H13; eauto |
+      rewrite Mem.upd_ne in H13; eauto].
+    {
+      cleanup.
+      unfold update_file, file_rep in *; simpl in *; cleanup.
+      eapply_fresh H11 in H7; eauto; cleanup.
+      intuition eauto.
+      rewrite length_updN; eauto.
+      eapply_fresh H14 in H15; cleanup.
+
+      destruct (addr_dec off i); subst.
+      {
+        eexists.
+        rewrite nth_error_updN_eq,
+        Mem.upd_eq; eauto.
+        eapply nth_error_nth in H15.
+        rewrite nth_selN_eq; eauto.
+        rewrite H13.
+        eapply nth_error_some_lt; eauto.
+      }
+      {
+        eexists.
+        rewrite nth_error_updN_ne,
+        Mem.upd_ne; eauto.
+        unfold inode_map_rep, inode_map_valid in *; cleanup.
+        apply H20 in H7; unfold inode_valid in *; cleanup.
+        eapply nth_error_nth in H15; rewrite <- H15.
+        rewrite <- nth_selN_eq; eauto.
+        eapply NoDup_selN_ne; eauto.
+        rewrite <- H13.
+        eapply nth_error_some_lt; eauto.
+      }
+    }
+    {
+      cleanup.
+      unfold update_file, file_rep in *; simpl in *; cleanup.
+      eapply_fresh H11 in H12; eauto; cleanup.
+      unfold file_rep; intuition eauto.
+      eapply_fresh H16 in H17; cleanup.
+      eexists; split; eauto.
+      rewrite Mem.upd_ne; eauto.
+
+      unfold inode_map_rep, inode_map_valid in *; cleanup.
+      eapply_fresh H23 in H12; eauto.           
+      apply nth_error_In in H17.
+      eapply not_In_NoDup_app in H17; eauto.
+      intros Hnot.
+      eapply selN_not_In_ne; eauto.
+    }
+  }
+}
+{
+  unfold file_map_rep; intuition eauto.
+}
+
+Unshelve.
+eauto. 
+Qed.
+  
+Lemma read_inner_finished:
+  forall u s s' o t inum off fm,
+    files_inner_rep fm (fst s) ->
+    exec (TransactionalDiskLang data_length) u o s (read_inner off inum) (Finished s' t) ->
+    files_inner_rep fm (fst s')
+    /\ snd s' = snd s.
+Proof.
+  unfold read_inner; intros; repeat invert_exec_no_match.
+  unfold files_rep, files_inner_rep in *; simpl in *; cleanup_no_match.
+  repeat cleanup_pairs.
+  eapply get_block_number_finished in H0; eauto.
+  simpl in *; cleanup_no_match; split_ors; cleanup_no_match;
+  repeat cleanup_pairs; repeat invert_exec_no_match;
+  eapply DiskAllocator.block_allocator_rep_inbounds_eq with (s2:= t1) in H2.
+  
+  eapply DiskAllocator.read_finished in H1; eauto.
+  simpl in *; cleanup_no_match; split_ors; cleanup_no_match;
+  repeat cleanup_pairs; repeat invert_exec_no_match;
+  
+  unfold inode_rep in *; cleanup_no_match;
+  eapply InodeAllocator.block_allocator_rep_inbounds_eq with (s2:= t2) in H1.
+
+  all: intros; repeat solve_bounds.
+  all: try solve [
+             simpl; repeat (split; eauto);
+             try eexists; intuition eauto ].
+Qed.
+
+(*** Crash Specs ***)
+
+
+
+Lemma auth_then_exec_crashed:
+  forall u o s s' inum T (p: Inum -> prog (TransactionalDiskLang data_length) (option T)) fm P,
+    files_rep fm s -> 
+    exec AuthenticatedDiskLang u o s (auth_then_exec inum p) (Crashed s') ->
+    (forall s s' o, 
+    files_inner_rep fm (fst s) ->
+    exec (TransactionalDiskLang data_length) u o s (p inum) (Crashed s') ->
+    snd s' = snd s) ->
+    forall fm',
+    (forall s s' o t, files_inner_rep fm (fst s) ->
+    exec (TransactionalDiskLang data_length) u o s (p inum) (Finished s' t) ->
+    ( t <> None -> 
+    files_inner_rep fm' (fst s') /\ P) /\ snd s' = snd s) ->    
+    files_crash_rep fm s' \/ 
+    (files_crash_rep fm' s' /\ 
+    P /\
+    exists f, 
+    inum < inode_count /\ 
+    fm inum = Some f /\ 
+    f.(BaseTypes.owner) = u).
+Proof.
+  unfold auth_then_exec,
+  files_rep, files_crash_rep; intros;
+  repeat (cleanup; repeat invert_exec; eauto;
+          try split_ors);
+  unfold files_inner_rep in *; cleanup; eauto;
+    repeat cleanup_pairs; simpl in *;
+    try eapply get_owner_crashed in H5; eauto;
+    try eapply get_owner_finished in H6; eauto;
+    try eapply H1 in H9; eauto;
+    try eapply H2 in H10; simpl in *; cleanup; eauto;
+    repeat cleanup_pairs; simpl in *; eauto;
+    try solve [left; eauto];
+    try solve [right; eauto];
+    try solve[
+    eexists; split; eauto;
+    eexists; split; eauto;
+    eapply DiskAllocator.block_allocator_rep_inbounds_eq; eauto;
+    intros; solve_bounds];
+    try solve [
+    right; edestruct H6; cleanup; 
+    try congruence; eexists; repeat (split; eauto); 
+    [intuition eauto |];
+    split_ors; cleanup;
+    eapply_fresh inode_rep_some_inbounds in H10; eauto;
+    eapply_fresh inode_exists_then_file_exists in H10; eauto; cleanup;
+    unfold file_map_rep, file_rep in *; cleanup;
+    eapply H14 in H10; eauto; cleanup; eexists; intuition eauto ].        
+Qed.
+
+Lemma read_inner_crashed:
+  forall u s s' o inum off fm,
+    files_inner_rep fm (fst s) ->
+    exec (TransactionalDiskLang data_length) u o s (read_inner off inum) (Crashed s') ->
+    snd s' = snd s.
+Proof.
+  unfold read_inner; intros; repeat invert_exec_no_match.
+  split_ors; cleanup; repeat invert_exec.
+  {
+    unfold files_rep, files_inner_rep in *; simpl in *; cleanup_no_match.
+    eapply get_block_number_crashed in H0; cleanup; eauto.
+  }
+
+  {
+    unfold files_rep, files_inner_rep in *; simpl in *; cleanup_no_match.
+    eapply get_block_number_finished in H0; cleanup; eauto;
+    repeat invert_exec; eauto.
+    {
+      repeat split_ors; cleanup.
+      {
+        eapply DiskAllocator.read_crashed in H1; eauto;
+        repeat cleanup_pairs; eauto.
+      }
+      {
+        eapply DiskAllocator.read_finished in H1; eauto; cleanup_no_match.
+        repeat cleanup_pairs; eauto.
+        2: {
+          clear H3.
+          eapply DiskAllocator.block_allocator_rep_inbounds_eq; eauto;
+          intros; solve_bounds. 
+        }
+        cleanup; repeat invert_exec; eauto.
+      }
+    }
+  }
+Qed.
+
+Lemma write_inner_crashed:
+  forall u s s' o inum off v fm,
+    files_inner_rep fm (fst s) ->
+    exec (TransactionalDiskLang data_length) u o s (write_inner off v inum) (Crashed s') ->
+    snd s' = snd s.
+Proof.
+  unfold write_inner; intros; repeat invert_exec_no_match.
+  split_ors; cleanup; repeat invert_exec.
+  {
+    unfold files_rep, files_inner_rep in *; simpl in *; cleanup_no_match.
+    eapply get_block_number_crashed in H0; cleanup; eauto.
+  }
+
+  {
+    unfold files_rep, files_inner_rep in *; simpl in *; cleanup_no_match.
+    eapply get_block_number_finished in H0; cleanup; eauto;
+    repeat invert_exec; eauto.
+    {
+      repeat split_ors; cleanup.
+      {
+        eapply DiskAllocator.write_crashed in H1; eauto;
+        repeat cleanup_pairs; eauto.
+      }
+    } 
+  }
+Qed.
+
+
+Lemma extend_inner_crashed:
+  forall u s s' o inum v fm,
+    files_inner_rep fm (fst s) ->
+    exec (TransactionalDiskLang data_length) u o s (extend_inner v inum) (Crashed s') ->
+    snd s' = snd s.
+Proof.
+  unfold extend_inner; intros; repeat invert_exec_no_match.
+  split_ors; cleanup; repeat invert_exec.
+  {
+    unfold files_rep, files_inner_rep in *; simpl in *; cleanup_no_match.
+    eapply DiskAllocator.alloc_crashed in H0; cleanup; eauto.
+  }
+
+  {
+    unfold files_rep, files_inner_rep in *; simpl in *; cleanup_no_match.
+    eapply DiskAllocator.alloc_finished in H0; cleanup; eauto;
+    repeat invert_exec; eauto.
+    {
+      repeat split_ors; cleanup.
+      {
+        eapply Inode.extend_crashed in H1; eauto;
+        repeat cleanup_pairs; eauto.
+        unfold inode_rep in *; cleanup.
+        eexists; intuition eauto.
+        eapply InodeAllocator.block_allocator_rep_inbounds_eq; eauto.
+        intros; repeat solve_bounds. 
+      }
+    } 
+  }
+Qed.
+
+Lemma free_all_blocks_crashed:
+  forall u l_a s s' o block_map,
+    DiskAllocator.block_allocator_rep block_map (fst s) ->
+    exec (TransactionalDiskLang data_length) u o s (free_all_blocks l_a) (Crashed s') ->
+    snd s' = snd s.
+Proof.
+  induction l_a; simpl; intros; repeat invert_exec_no_match; eauto.
+  split_ors; cleanup; repeat invert_exec.
+  {
+    unfold files_rep, files_inner_rep in *; simpl in *; cleanup_no_match.
+    eapply DiskAllocator.free_crashed in H0; cleanup; eauto.
+  }
+
+  {
+    unfold files_rep, files_inner_rep in *; simpl in *; cleanup_no_match.
+    eapply DiskAllocator.free_finished in H0; cleanup; eauto;
+    repeat invert_exec; eauto;
+    repeat split_ors; cleanup; eauto.
+    repeat cleanup_pairs; eapply IHl_a in H1; eauto.
+  }
+Qed.
+
+Lemma delete_inner_crashed:
+  forall u s s' o inum fm,
+    files_inner_rep fm (fst s) ->
+    exec (TransactionalDiskLang data_length) u o s (delete_inner inum) (Crashed s') ->
+    snd s' = snd s.
+Proof.
+  unfold delete_inner; intros; repeat invert_exec_no_match.
+  split_ors; cleanup; repeat invert_exec.
+  {
+    unfold files_rep, files_inner_rep in *; simpl in *; cleanup_no_match.
+    eapply get_all_block_numbers_crashed in H0; cleanup; eauto.
+  }
+
+  {
+    unfold files_rep, files_inner_rep in *; simpl in *; cleanup_no_match.
+    eapply get_all_block_numbers_finished in H0; cleanup; eauto;
+    repeat invert_exec; eauto.
+    {
+      repeat split_ors; cleanup.
+      {
+        repeat cleanup_pairs.
+        eapply free_all_blocks_crashed in H1; eauto;
+        repeat cleanup_pairs; eauto.
+        clear H3; simpl; eapply DiskAllocator.block_allocator_rep_inbounds_eq; eauto.
+        intros; repeat solve_bounds.
+      }
+      repeat cleanup_pairs; simpl in *.
+      eapply free_all_blocks_finished in H1; simpl; eauto.
+      2: simpl; eapply DiskAllocator.block_allocator_rep_inbounds_eq; eauto;
+        intros; repeat solve_bounds.
+      simpl in *; cleanup; split_ors; cleanup;
+      repeat invert_exec; eauto.
+      eapply free_crashed in H8; eauto.
+    } 
+  }
+Qed.
+
+Lemma change_owner_inner_crashed:
+  forall u s s' o inum own fm,
+    files_inner_rep fm (fst s) ->
+    exec (TransactionalDiskLang data_length) u o s (change_owner_inner own inum) (Crashed s') ->
+    snd s' = snd s.
+Proof.
+  unfold change_owner_inner; intros; repeat invert_exec_no_match.
+  unfold files_rep, files_inner_rep in *; simpl in *; cleanup_no_match.
+  eapply Inode.change_owner_crashed in H0; cleanup; eauto.
+Qed.
